vale/code/lib/transformers/Vale.Transformers.PeepHole.fsti
@@ -6,14 +6,11 @@
    [peephole], and an [input_hint] to obtain a new transformer.
 
    A [peephole] is a function that converts a list of instructions
-   into (optionally) another list of instructions. It must be proven
-   correct wrt preservation of semantics. The [input_hint] is just a
-   hint to say how many instructions it takes as input.
+   into (optionally) another list of instructions.
 
    Usage:
-
-     let test = peephole_transform test_ih test_ph
-     let lemma_test = lemma_peephole_transform test_ih test_ph
+     let foo = peephole_transform foo_ph
+     let lemma_foo = lemma_peephole_transform foo_ph
 
 *)
 module Vale.Transformers.PeepHole
@@ -43,7 +40,11 @@ open Vale.X64.InsLemmas
 
 /// Define what a peephole means, and what it means to be correct.
 
-type pre_peephole = list ins -> Tot (option (list ins))
+noeq
+type pre_peephole = {
+  ph: list ins -> Tot (option (list ins)); // The actual peephole transformer
+  input_hint: pos; // The number of instructions it takes as input to transform
+}
 
 let rec eval_inss (is:list ins) (s:machine_state) : GTot machine_state =
   match is with
@@ -51,7 +52,7 @@ let rec eval_inss (is:list ins) (s:machine_state) : GTot machine_state =
   | i :: is' -> eval_inss is' (machine_eval_ins i s)
 
 let peephole_correct (p:pre_peephole) (is:list ins) (s:machine_state) : GTot Type0 =
-  match p is with
+  match p.ph is with
   | None -> True
   | Some is' ->
     equiv_states_or_both_not_ok
@@ -65,18 +66,18 @@ type peephole = (p:pre_peephole{forall is s. {:pattern (peephole_correct p is s)
 /// something you can directly use as transformers!
 
 val peephole_transform :
-  input_hint:pos -> p:peephole ->
+  p:peephole ->
   orig:va_code ->
   va_transformation_result
 
 val lemma_peephole_transform :
-  input_hint:pos -> p:peephole ->
+  p:peephole ->
   orig:va_code ->
   transformed:va_code ->
   va_s0:va_state -> va_sM:va_state -> va_fM:va_fuel ->
   Ghost (va_state & va_fuel)
     (requires (
-        (va_require_total transformed (peephole_transform input_hint p orig).result va_s0) /\
+        (va_require_total transformed (peephole_transform p orig).result va_s0) /\
         (va_get_ok va_s0) /\
         (va_ensure_total orig va_s0 va_sM va_fM) /\
         (va_get_ok va_sM)))
